

Задание 5

$$\textcircled{1} \quad \lim_{x \rightarrow 1} \frac{\sqrt{x^2 + 2x + 6} - \sqrt{x^2 + 3x + 5}}{x - 1} = \left(\frac{0}{0} \right) =$$

$$= \lim_{x \rightarrow 1} \frac{(\sqrt{x^2 + 2x + 6} - \sqrt{x^2 + 3x + 5})(\sqrt{x^2 + 2x + 6} + \sqrt{x^2 + 3x + 5})}{(x - 1)(\sqrt{x^2 + 2x + 6} + \sqrt{x^2 + 3x + 5})} =$$

$$= \lim_{x \rightarrow 1} \frac{x^2 + 2x + 6 - x^2 - 3x - 5}{(x - 1)(\sqrt{x^2 + 2x + 6} + \sqrt{x^2 + 3x + 5})} =$$

$$= \lim_{x \rightarrow 1} \frac{-(x - 1)}{(x - 1)(\sqrt{x^2 + 2x + 6} + \sqrt{x^2 + 3x + 5})} =$$

$$= \lim_{x \rightarrow 1} \frac{-1}{\sqrt{x^2 + 2x + 6} + \sqrt{x^2 + 3x + 5}} = \frac{-1}{\sqrt{9} + \sqrt{9}} = -\frac{1}{6}$$

$$\textcircled{2} \quad \lim_{x \rightarrow 0} \frac{5 \ln(1 + 5x) \arcsin 4x}{1 - \cos 2x} =$$

$$= \lim_{x \rightarrow 0} \frac{5 \cdot 5x \cdot 4x \cdot 2}{(2x)^2} = 50$$